<?xml version="1.0" encoding="UTF-8"?>
<rdf:RDF xmlns:cc="http://creativecommons.org/ns#" xmlns:dc="http://purl.org/dc/elements/1.1/"
    xmlns:dcterms="http://purl.org/dc/terms/" xmlns:html="http://www.w3.org/1999/xhtml"
    xmlns:owl="http://www.w3.org/2002/07/owl#"
    xmlns:rdf="http://www.w3.org/1999/02/22-rdf-syntax-ns#"
    xmlns:rdfs="http://www.w3.org/2000/01/rdf-schema#"
    xmlns:ric-dft="https://www.ica.org/standards/RiC/vocabularies/documentaryFormTypes#"
    xmlns:ric-rst="https://www.ica.org/standards/RiC/vocabularies/recordSetTypes#"
    xmlns:rico="https://www.ica.org/standards/RiC/ontology#"
    xmlns:skos="http://www.w3.org/2004/02/skos/core#" xmlns:vann="http://purl.org/vocab/vann/"
    xmlns:voaf="http://purl.org/vocommons/voaf#"
    xmlns:xs="http://www.w3.org/2001/XMLSchema">

    <skos:ConceptScheme
        rdf:about="https://www.ica.org/standards/RiC/vocabularies/documentaryFormTypes">
        <rdfs:label xml:lang="en">Documentary Form Types</rdfs:label>
        <rdfs:label xml:lang="fr">Types de documents</rdfs:label>
        <rdfs:label xml:lang="es">Tipos documentales</rdfs:label>
        <dc:title xml:lang="en">International Council on Archives Records in Contexts Vocabulary for
Documentary Form Types</dc:title>
        <cc:license rdf:resource="https://creativecommons.org/licenses/by/4.0/"/>
        <dc:contributor xml:lang="en">Florence Clavaud (Archives nationales de France), member of
            EGAD and lead of EGAD RiC-O team from 2012</dc:contributor>
        <dc:contributor>Regine I. Heberlein (University of Princeton, USA), member of EGAD and EGAD
            RiC-O team from 2023</dc:contributor>
        <dc:contributor xml:lang="en">Miia Herrala (National Archives of Finland), member of EGAD
            and EGAD RiC-O team from 2016 to 2022</dc:contributor>
        <dc:contributor xml:lang="en">Jan Krause-Bilvin (docuteam, Switzerland),
            member of EGAD and EGAD RiC-O team from 2023</dc:contributor>
        <dc:contributor xml:lang="en">Daniel Pitti (University of Virginia, USA), chair of EGAD from
            2012</dc:contributor>
        <dc:contributor xml:lang="en">Aaron Rubinstein (University of Massachusetts Amherst, USA),
            member of EGAD and EGAD RiC-O team from 2012 to 2022</dc:contributor>
        <dc:contributor xml:lang="en">Tobias Wildi (docuteam, Switzerland), member of EGAD and EGAD RiC-O team from 2019</dc:contributor>
        <dc:contributor xml:lang="en">Richard David Williamson (National Archives of Norway), member
            of EGAD and of EGAD RiC-O team from 2024</dc:contributor>
        <dc:contributor xml:lang="en">Ivo Zandhuis (Consultant Digital Cultural Heritage, The
            Netherlands), member of EGAD and EGAD RiC-O team from 2023</dc:contributor>
        <!-- ORCID links for the current members of EGAD -->
        <dcterms:contributor rdf:resource="https://orcid.org/0000-0002-5681-4850"/>
        <dcterms:contributor rdf:resource="https://orcid.org/0000-0002-0803-8025"/>
        <dcterms:contributor rdf:resource="https://orcid.org/0000-0001-9375-2102"/>
        <dcterms:contributor rdf:resource="https://orcid.org/0000-0001-9938-6502"/>
        <dcterms:contributor rdf:resource="https://orcid.org/0000-0001-6743-9622"/>
        <dcterms:contributor rdf:resource="https://orcid.org/0009-0004-3219-2534"/>
        <dcterms:contributor rdf:resource="https://orcid.org/0000-0003-0165-8341"/>
        <dc:creator xml:lang="en">International Council on Archives Expert Group on Archival
            Description (ICA EGAD)</dc:creator>
        <dc:publisher xml:lang="en">International Council on Archives</dc:publisher>
        <dc:rights xml:lang="en">Copyright 2019-, International Council on Archives
            (ICA)</dc:rights>
        <skos:definition xml:lang="en">A vocabulary that provides URIs for describing documentary
            form types of RiC Records and Record Parts.</skos:definition>
        <dc:language>en</dc:language>
        <dc:language>fr</dc:language>
        <dc:language>es</dc:language>

        <skos:historyNote xml:lang="en">This vocabulary was created within the Records in Contexts
            Ontology. When the ICA/EGAD developed RiC-O 1.0, it was decided that two versions of RiC-O
            would be released. The first one, consisting of a unique large OWL file, would remain the
            reference one. RiC-0 1.0 would also be provided as a set of files, in order to address
            specific needs, e.g. using only the core of the ontology, or using only the individuals it
            defined and defining new individuals. So from December 2023, you can find the vocabulary on
            Documentary Form Types, either in the unique large OWL RiC-O file, or as a separate file. </skos:historyNote>
        <skos:changeNote
            >
            <rdf:Description>
                <dc:date>2024-05-13</dc:date>
                <rdf:value xml:lang="en">Added the name and ORCID of Richard Williamson to the contributors, changed the affiliation of J. Krause-Bilvin and T. Wildi.</rdf:value>
            </rdf:Description>
        </skos:changeNote>
        <skos:changeNote
            >
            <rdf:Description>
                <dc:date>2023-12-13</dc:date>
                <rdf:value xml:lang="en">Completed the metadata of the vocabulary: added dc:language, a history note and a scope note.</rdf:value>
            </rdf:Description>
        </skos:changeNote>
        <skos:changeNote>
            <rdf:Description>
                <dc:date>2023-11-25</dc:date>
                <rdf:value xml:lang="en">Added a new rdfs:label in Spanish.</rdf:value>
            </rdf:Description>
        </skos:changeNote>
        <skos:changeNote>
            <rdf:Description>
                <dc:date>2023-08-28</dc:date>
                <rdf:value xml:lang="en">Added a new rdfs:label in French.</rdf:value>
            </rdf:Description>
        </skos:changeNote>
        <skos:scopeNote xml:lang="en">For now this vocabulary only defines two top concepts; it should
            hopefully be completed later. The concepts defined in this vocabulary can be used in
            combination with RiC-O classes and properties, whenever necessary and appropriate, to
            assign a documentary form type to a Record or a Record Part, using the
            rico:hasDocumentaryFormType object property, or its inverse one. They also can be used
            to specify that a rico:RecordSet included or includes members whose some
            (rico:hasOrHadSomeMembersWithDocumentaryFormType) or all
            (rico:hasOrHadAllMembersWithDocumentaryFormType) have some Documentary Form Type. Each
            concept is both defined as a skos:Concept and a rico:DocumentaryFormType, so that it is
            possible to extend the classic definition of such concepts using RiC-O properties. For
            example, you can use rico:history, rico:date, or rico:isAssociatedWithPlace,
            rico:precedesInTime, if you consider a documentary form type as being a historical
            entity, known and used in some known space or time region.</skos:scopeNote>
        <skos:hasTopConcept
            rdf:resource="https://www.ica.org/standards/RiC/vocabularies/documentaryFormTypes#AuthorityRecord"/>
        <skos:hasTopConcept
            rdf:resource="https://www.ica.org/standards/RiC/vocabularies/documentaryFormTypes#FindingAid"
        />
    </skos:ConceptScheme>
    <!-- https://www.ica.org/standards/RiC/vocabularies/documentaryFormTypes#AuthorityRecord -->
    <skos:Concept
        rdf:about="https://www.ica.org/standards/RiC/vocabularies/documentaryFormTypes#AuthorityRecord">
        <rdf:type rdf:resource="https://www.ica.org/standards/RiC/ontology#DocumentaryFormType"/>
        <rdfs:label xml:lang="en">authority record</rdfs:label>
        <rdfs:label xml:lang="fr">notice d’autorité</rdfs:label>
        <rdfs:label xml:lang="es">registro de autoridad</rdfs:label>
        <skos:changeNote>
            <rdf:Description>
                <dc:date>2023-11-25</dc:date>
                <rdf:value xml:lang="en">Added a new rdfs:label in Spanish.</rdf:value>
            </rdf:Description>
        </skos:changeNote>
        <skos:changeNote>
            <rdf:Description>
                <dc:date>2023-08-28</dc:date>
                <rdf:value xml:lang="en">Added a new rdfs:label in French.</rdf:value>
            </rdf:Description>
        </skos:changeNote>
        <skos:definition xml:lang="en">This category can be used for records that describe an
            entity.</skos:definition>
        <skos:inScheme
            rdf:resource="https://www.ica.org/standards/RiC/vocabularies/documentaryFormTypes"/>
        <skos:topConceptOf
            rdf:resource="https://www.ica.org/standards/RiC/vocabularies/documentaryFormTypes"/>
    </skos:Concept>
    <!-- https://www.ica.org/standards/RiC/vocabularies/documentaryFormTypes#FindingAid -->
    <skos:Concept
        rdf:about="https://www.ica.org/standards/RiC/vocabularies/documentaryFormTypes#FindingAid">
        <rdf:type rdf:resource="https://www.ica.org/standards/RiC/ontology#DocumentaryFormType"/>
        <rdfs:label xml:lang="en">finding aid</rdfs:label>
        <rdfs:label xml:lang="fr">instrument de recherche</rdfs:label>
        <rdfs:label xml:lang="es">instrumento de descripción</rdfs:label>
        <skos:changeNote>
            <rdf:Description>
                <dc:date>2023-11-25</dc:date>
                <rdf:value xml:lang="en">Added a new rdfs:label in Spanish.</rdf:value>
            </rdf:Description>
        </skos:changeNote>
        <skos:changeNote>
            <rdf:Description>
                <dc:date>2023-08-28</dc:date>
                <rdf:value xml:lang="en">Added a new rdfs:label in French.</rdf:value>
            </rdf:Description>
        </skos:changeNote>
        <skos:definition xml:lang="en">This documentary form type can be used for records that
            aggregate and organize metadata on some record(s) or record set(s).</skos:definition>
        <skos:inScheme
            rdf:resource="https://www.ica.org/standards/RiC/vocabularies/documentaryFormTypes"/>
        <skos:topConceptOf
            rdf:resource="https://www.ica.org/standards/RiC/vocabularies/documentaryFormTypes"/>
    </skos:Concept>
    <owl:Class rdf:about="https://www.ica.org/standards/RiC/ontology#DocumentaryFormType">
        <rdfs:isDefinedBy rdf:resource="https://www.ica.org/standards/RiC/ontology"/>
    </owl:Class>
</rdf:RDF>
