<?xml version="1.0" encoding="UTF-8"?>
<rdf:RDF xmlns:cc="http://creativecommons.org/ns#" xmlns:dc="http://purl.org/dc/elements/1.1/"
    xmlns:dcterms="http://purl.org/dc/terms/" xmlns:html="http://www.w3.org/1999/xhtml"
    xmlns:owl="http://www.w3.org/2002/07/owl#"
    xmlns:rdf="http://www.w3.org/1999/02/22-rdf-syntax-ns#"
    xmlns:rdfs="http://www.w3.org/2000/01/rdf-schema#"
    xmlns:ric-dft="https://www.ica.org/standards/RiC/vocabularies/documentaryFormTypes#"
    xmlns:ric-rst="https://www.ica.org/standards/RiC/vocabularies/recordSetTypes#"
    xmlns:rico="https://www.ica.org/standards/RiC/ontology#"
    xmlns:skos="http://www.w3.org/2004/02/skos/core#" xmlns:vann="http://purl.org/vocab/vann/"
    xmlns:voaf="http://purl.org/vocommons/voaf#"
    xmlns:xs="http://www.w3.org/2001/XMLSchema">
    
    <skos:ConceptScheme
        rdf:about="https://www.ica.org/standards/RiC/vocabularies/recordSetTypes">
        <rdfs:label xml:lang="en">Record Set Types</rdfs:label>
        <rdfs:label xml:lang="fr">Types d’ensembles d’objets informationnels</rdfs:label>
        <rdfs:label xml:lang="es">Tipos de agrupación documental</rdfs:label>
        <dc:title xml:lang="en">International Council on Archives Records in Contexts Vocabulary for
            Record Set Types</dc:title>
        <cc:license rdf:resource="https://creativecommons.org/licenses/by/4.0/"/>
        <dc:contributor xml:lang="en">Florence Clavaud (Archives nationales de France), member of
            EGAD and lead of EGAD RiC-O team from 2012</dc:contributor>
        <dc:contributor>Regine I. Heberlein (University of Princeton, USA), member of EGAD and EGAD
            RiC-O team from 2023</dc:contributor>
        <dc:contributor xml:lang="en">Miia Herrala (National Archives of Finland), member of EGAD
            and EGAD RiC-O team from 2016 to 2022</dc:contributor>
        <dc:contributor xml:lang="en">Jan Krause-Bilvin (Archives cantonales vaudoises,
            Switzerland), member of EGAD and EGAD RiC-O team from 2023</dc:contributor>
        <dc:contributor xml:lang="en">Daniel Pitti (University of Virginia, USA), chair of EGAD from
            2012</dc:contributor>
        <dc:contributor xml:lang="en">Aaron Rubinstein (University of Massachusetts Amherst, USA),
            member of EGAD and EGAD RiC-O team from 2012 to 2022</dc:contributor>
        <dc:contributor xml:lang="en">Tobias Wildi (University of Applied Sciences of the Grisons,
            Switzerland), member of EGAD and EGAD RiC-O team from 2019</dc:contributor>
        <dc:contributor xml:lang="en">Ivo Zandhuis (Consultant Digital Cultural Heritage, The
            Netherlands), member of EGAD and EGAD RiC-O team from 2023</dc:contributor>
        <!-- ORCID links for the current members of EGAD -->
        <dcterms:contributor rdf:resource="https://orcid.org/0000-0002-5681-4850"/>
        <dcterms:contributor rdf:resource="https://orcid.org/0000-0002-0803-8025"/>
        <dcterms:contributor rdf:resource="https://orcid.org/0000-0001-9375-2102"/>
        <dcterms:contributor rdf:resource="https://orcid.org/0000-0001-9938-6502"/>
        <dcterms:contributor rdf:resource="https://orcid.org/0000-0001-6743-9622"/>
        <dcterms:contributor rdf:resource="https://orcid.org/0000-0003-0165-8341"/>
        <dc:creator xml:lang="en">International Council on Archives Expert Group on Archival
            Description (ICA EGAD)</dc:creator>
        <dc:publisher xml:lang="en">International Council on Archives</dc:publisher>
        <dc:rights xml:lang="en">Copyright 2019-, International Council on Archives
            (ICA)</dc:rights>
        <skos:definition xml:lang="en">A vocabulary that provides URIs for describing types
            of RiC Record Sets.</skos:definition>
        <dc:language>en</dc:language>
        <dc:language>fr</dc:language>
        <dc:language>es</dc:language>
        <skos:historyNote xml:lang="en">This vocabulary was created within the Records in Contexts
            Ontology. When the ICA/EGAD developed RiC-O 1.0, it was decided that two versions of RiC-O
            would be released. The first one, consisting of a unique large OWL file, would remain the
            reference one. RiC-0 1.0 would also be provided as a set of files, in order to address
            specific needs, e.g. using only the core of the ontology, or using only the individuals it
            defined and defining new individuals. So from December 2023, you can find the vocabulary on
            Record Set Types, either in the unique large OWL RiC-O file, or as a separate file. </skos:historyNote>
        <skos:changeNote
            >
            <rdf:Description>
                <dc:date>2023-12-13</dc:date>
                <rdf:value xml:lang="en">Completed the metadata of the vocabulary: added dc:language, a history note and a scope note.</rdf:value>
            </rdf:Description>
        </skos:changeNote>
        <skos:changeNote>
            <rdf:Description>
                <dc:date>2023-11-25</dc:date>
                <rdf:value xml:lang="en">Added a new rdfs:label in Spanish.</rdf:value>
            </rdf:Description>
        </skos:changeNote>
        <skos:changeNote>
            <rdf:Description>
                <dc:date>2023-08-28</dc:date>
                <rdf:value xml:lang="en">Added a new rdfs:label in French.</rdf:value>
            </rdf:Description>
        </skos:changeNote>
        <skos:scopeNote xml:lang="en">For now this vocabulary only defines four top concepts; it
            should hopefully be completed later. The concepts defined in this vocabulary can be used in
            combination with RiC-O classes and properties, whenever necessary and appropriate, to
            assign a record set type to a Record Set, using the rico:hasRecordSetType object property,
            or its inverse one. Each concept is both defined as a skos:Concept and a
            rico:RecordSetType, so that it is possible to extend the classic definition of such
            concepts using RiC-O properties. For example, you can use rico:history, rico:date, or
            rico:isAssociatedWithPlace, rico:precedesInTime, if you consider a record set type as being
            a historical entity, known and used in some known space or time region.</skos:scopeNote>
      
        
      
        <skos:hasTopConcept
            rdf:resource="https://www.ica.org/standards/RiC/vocabularies/recordSetTypes#Collection"/>
        <skos:hasTopConcept
            rdf:resource="https://www.ica.org/standards/RiC/vocabularies/recordSetTypes#File"
        />
        <skos:hasTopConcept rdf:resource="https://www.ica.org/standards/RiC/vocabularies/recordSetTypes#Fonds"/>
        <skos:hasTopConcept rdf:resource="https://www.ica.org/standards/RiC/vocabularies/recordSetTypes#Series"/>
    </skos:ConceptScheme>
    <!-- https://www.ica.org/standards/RiC/vocabularies/recordSetTypes#Collection -->
    <skos:Concept rdf:about="https://www.ica.org/standards/RiC/vocabularies/recordSetTypes#Collection">
        <rdf:type rdf:resource="https://www.ica.org/standards/RiC/ontology#RecordSetType"/>
        <rdfs:label xml:lang="en">collection</rdfs:label>
        <rdfs:label xml:lang="fr">collection</rdfs:label>
        <rdfs:label xml:lang="es">colección</rdfs:label>
        <skos:changeNote>
            <rdf:Description>
                <dc:date>2023-11-25</dc:date>
                <rdf:value xml:lang="en">Added a new rdfs:label in Spanish.</rdf:value>
            </rdf:Description>
        </skos:changeNote>
        <skos:changeNote>
            <rdf:Description>
                <dc:date>2023-08-28</dc:date>
                <rdf:value xml:lang="en">Added a new rdfs:label in French.</rdf:value>
            </rdf:Description>
        </skos:changeNote>
        <skos:definition xml:lang="en">An artificial assemblage of documents accumulated on the
            basis of some common characteristic without regard to the provenance of those documents.
            Not to be confused with an archival fonds. (From ICA ISAD(G))</skos:definition>
        <skos:inScheme rdf:resource="https://www.ica.org/standards/RiC/vocabularies/recordSetTypes"/>
        <skos:topConceptOf rdf:resource="https://www.ica.org/standards/RiC/vocabularies/recordSetTypes"/>
        </skos:Concept>
    <!-- https://www.ica.org/standards/RiC/vocabularies/recordSetTypes#File -->
    <skos:Concept rdf:about="https://www.ica.org/standards/RiC/vocabularies/recordSetTypes#File">
        <rdf:type rdf:resource="https://www.ica.org/standards/RiC/ontology#RecordSetType"/>
        <rdfs:label xml:lang="fr">dossier</rdfs:label>
        <rdfs:label xml:lang="en">file</rdfs:label>
        <rdfs:label xml:lang="es">expediente</rdfs:label>
        <skos:changeNote>
            <rdf:Description>
                <dc:date>2023-11-25</dc:date>
                <rdf:value xml:lang="en">Added a new rdfs:label in Spanish.</rdf:value>
            </rdf:Description>
        </skos:changeNote>
        <skos:changeNote>
            <rdf:Description>
                <dc:date>2023-08-28</dc:date>
                <rdf:value xml:lang="en">Added a new rdfs:label in French.</rdf:value>
            </rdf:Description>
        </skos:changeNote>
        <skos:definition xml:lang="en">An organized unit of documents grouped together either for
            current use by the creator or in the process of archival arrangement, because they
            relate to the same subject, activity, or transaction. A file is usually the basic unit
            within a record series. (From ICA ISAD(G))</skos:definition>
        <skos:inScheme rdf:resource="https://www.ica.org/standards/RiC/vocabularies/recordSetTypes"/>
        <skos:topConceptOf rdf:resource="https://www.ica.org/standards/RiC/vocabularies/recordSetTypes"/>
        </skos:Concept>
    <!-- https://www.ica.org/standards/RiC/vocabularies/recordSetTypes#Fonds -->
       <skos:Concept rdf:about="https://www.ica.org/standards/RiC/vocabularies/recordSetTypes#Fonds">
        <rdf:type rdf:resource="http://www.w3.org/2004/02/skos/core#Concept"/>
        <rdf:type rdf:resource="https://www.ica.org/standards/RiC/ontology#RecordSetType"/>
        <rdfs:label xml:lang="en">fonds</rdfs:label>
        <rdfs:label xml:lang="fr">fonds</rdfs:label>
        <rdfs:label xml:lang="es">fondo</rdfs:label>
        <skos:changeNote>
            <rdf:Description>
                <dc:date>2023-11-25</dc:date>
                <rdf:value xml:lang="en">Added a new rdfs:label in Spanish.</rdf:value>
            </rdf:Description>
        </skos:changeNote>
        <skos:changeNote>
            <rdf:Description>
                <dc:date>2023-08-28</dc:date>
                <rdf:value xml:lang="en">Added a new rdfs:label in French.</rdf:value>
            </rdf:Description>
        </skos:changeNote>
        <skos:definition xml:lang="en">The whole of the records, regardless of form or medium,
            organically created and/or accumulated and used by a particular person, family, or
            corporate body in the course of that creator's activities and functions. (From ICA
            ISAD(G))</skos:definition>
        <skos:inScheme rdf:resource="https://www.ica.org/standards/RiC/vocabularies/recordSetTypes"/>
        <skos:topConceptOf rdf:resource="https://www.ica.org/standards/RiC/vocabularies/recordSetTypes"/>
    </skos:Concept>
    <!-- https://www.ica.org/standards/RiC/vocabularies/recordSetTypes#Series -->
    <skos:Concept rdf:about="https://www.ica.org/standards/RiC/vocabularies/recordSetTypes#Series">
        <rdf:type rdf:resource="http://www.w3.org/2004/02/skos/core#Concept"/>
        <rdf:type rdf:resource="https://www.ica.org/standards/RiC/ontology#RecordSetType"/>
        <rdfs:label xml:lang="en">series</rdfs:label>
        <rdfs:label xml:lang="fr">série organique</rdfs:label>
        <rdfs:label xml:lang="es">serie</rdfs:label>
        <skos:changeNote>
            <rdf:Description>
                <dc:date>2023-11-25</dc:date>
                <rdf:value xml:lang="en">Added a new rdfs:label in Spanish.</rdf:value>
            </rdf:Description>
        </skos:changeNote>
        <skos:changeNote>
            <rdf:Description>
                <dc:date>2023-08-28</dc:date>
                <rdf:value xml:lang="en">Added a new rdfs:label in French.</rdf:value>
            </rdf:Description>
        </skos:changeNote>
        <skos:definition xml:lang="en">Documents arranged in accordance with a filing system or
            maintained as a unit because they result from the same accumulation or filing process,
            or the same activity; have a particular form; or because of some other relationship
            arising out of their creation, receipt, or use. A series is also known as a records
            series. (From ICA ISAD(G))</skos:definition>
        <skos:inScheme rdf:resource="https://www.ica.org/standards/RiC/vocabularies/recordSetTypes"/>
        <skos:topConceptOf rdf:resource="https://www.ica.org/standards/RiC/vocabularies/recordSetTypes"/>
    </skos:Concept>
    <owl:Class rdf:about="https://www.ica.org/standards/RiC/ontology#RecordSetType">
        <rdfs:isDefinedBy rdf:resource="https://www.ica.org/standards/RiC/ontology"/>
    </owl:Class>
</rdf:RDF>